src/Std/Tactic/BVDecide/Bitblast/BVExpr/Circuit/Impl/Expr.lean
@@ -3,7 +3,6 @@ Copyright (c) 2024 Lean FRO, LLC. All rights reserved.
 Released under Apache 2.0 license as described in the file LICENSE.
 Authors: Henrik Böving
 -/
-module
 
 prelude
 public import Std.Tactic.BVDecide.Bitblast.BVExpr.Circuit.Impl.Var
@@ -17,6 +16,7 @@ public import Std.Tactic.BVDecide.Bitblast.BVExpr.Circuit.Impl.Operations.Mul
 public import Std.Tactic.BVDecide.Bitblast.BVExpr.Circuit.Impl.Operations.Umod
 public import Std.Tactic.BVDecide.Bitblast.BVExpr.Circuit.Impl.Operations.Reverse
 public import Std.Tactic.BVDecide.Bitblast.BVExpr.Circuit.Impl.Operations.Clz
+import Std.Tactic.BVDecide.Bitblast.BVExpr.Circuit.Impl.Operations.PopCount
 
 @[expose] public section
 
@@ -230,8 +230,8 @@ where
           apply AIG.LawfulVecOperator.le_size_of_le_aig_size (f := bitblast.blastClz)
           omega
         ⟨⟨res, this⟩, cache.cast (AIG.LawfulVecOperator.le_size (f := bitblast.blastClz) ..)⟩
-      | .popCnt => sorry
-        -- let res := bitblast.blastPopCnt eaig evec
+      | .popCount => sorry
+        -- let res := bitblast.blastPopCount eaig evec
         -- have := by
         --   apply AIG.LawfulVecOperator.le_size_of_le_aig_size (f := bitblast.blastClz)
         --   omega
