src/Std/Tactic/BVDecide/Bitblast/BVExpr/Circuit/Lemmas/Expr.lean
@@ -6,21 +6,25 @@ Authors: Henrik Böving
 module
 
 prelude
-public import Std.Tactic.BVDecide.Bitblast.BVExpr.Circuit.Lemmas.Var
-public import Std.Tactic.BVDecide.Bitblast.BVExpr.Circuit.Lemmas.Operations.ShiftRight
-public import Std.Tactic.BVDecide.Bitblast.BVExpr.Circuit.Lemmas.Operations.Append
-public import Std.Tactic.BVDecide.Bitblast.BVExpr.Circuit.Lemmas.Operations.Replicate
-public import Std.Tactic.BVDecide.Bitblast.BVExpr.Circuit.Lemmas.Operations.Extract
-public import Std.Tactic.BVDecide.Bitblast.BVExpr.Circuit.Lemmas.Operations.RotateLeft
-public import Std.Tactic.BVDecide.Bitblast.BVExpr.Circuit.Lemmas.Operations.RotateRight
-public import Std.Tactic.BVDecide.Bitblast.BVExpr.Circuit.Lemmas.Operations.Mul
-public import Std.Tactic.BVDecide.Bitblast.BVExpr.Circuit.Lemmas.Operations.Umod
-public import Std.Tactic.BVDecide.Bitblast.BVExpr.Circuit.Lemmas.Operations.Reverse
-public import Std.Tactic.BVDecide.Bitblast.BVExpr.Circuit.Lemmas.Operations.Clz
-public import Std.Tactic.BVDecide.Bitblast.BVExpr.Circuit.Lemmas.Operations.PopCount
-public import Std.Tactic.BVDecide.Bitblast.BVExpr.Circuit.Impl.Expr
-
-@[expose] public section
+import Std.Tactic.BVDecide.Bitblast.BVExpr.Circuit.Lemmas.Basic
+import Std.Tactic.BVDecide.Bitblast.BVExpr.Circuit.Lemmas.Const
+import Std.Tactic.BVDecide.Bitblast.BVExpr.Circuit.Lemmas.Var
+import Std.Tactic.BVDecide.Bitblast.BVExpr.Circuit.Lemmas.Operations.Not
+import Std.Tactic.BVDecide.Bitblast.BVExpr.Circuit.Lemmas.Operations.ShiftLeft
+import Std.Tactic.BVDecide.Bitblast.BVExpr.Circuit.Lemmas.Operations.ShiftRight
+import Std.Tactic.BVDecide.Bitblast.BVExpr.Circuit.Lemmas.Operations.Add
+import Std.Tactic.BVDecide.Bitblast.BVExpr.Circuit.Lemmas.Operations.Append
+import Std.Tactic.BVDecide.Bitblast.BVExpr.Circuit.Lemmas.Operations.Replicate
+import Std.Tactic.BVDecide.Bitblast.BVExpr.Circuit.Lemmas.Operations.Extract
+import Std.Tactic.BVDecide.Bitblast.BVExpr.Circuit.Lemmas.Operations.RotateLeft
+import Std.Tactic.BVDecide.Bitblast.BVExpr.Circuit.Lemmas.Operations.RotateRight
+import Std.Tactic.BVDecide.Bitblast.BVExpr.Circuit.Lemmas.Operations.Mul
+import Std.Tactic.BVDecide.Bitblast.BVExpr.Circuit.Lemmas.Operations.Udiv
+import Std.Tactic.BVDecide.Bitblast.BVExpr.Circuit.Lemmas.Operations.Umod
+import Std.Tactic.BVDecide.Bitblast.BVExpr.Circuit.Lemmas.Operations.Reverse
+import Std.Tactic.BVDecide.Bitblast.BVExpr.Circuit.Lemmas.Operations.Clz
+import Std.Tactic.BVDecide.Bitblast.BVExpr.Circuit.Lemmas.Operations.PopCount
+import Std.Tactic.BVDecide.Bitblast.BVExpr.Circuit.Impl.Expr
 
 /-!
 This module contains the verification of the `BitVec` expressions (`BVExpr`) bitblaster from
